\documentclass{article}
\usepackage{epsfig}
\pagestyle{empty}
\begin{document}
$f$
\pagebreak

$g$
\pagebreak

$ f \circ g $
\pagebreak

$ f(x)=x $
\pagebreak

$ d_0 j^2 + d_1 \log(j),\ j=\det(A) $
\pagebreak

$ d_0 j^5 + d_1 j^{-5},\ j=\det(A) $
\pagebreak

$ \frac{\beta}{3}\iota_1(\sigma) + J_2(\sigma)-offset $
\pagebreak

$\iota_1$
\pagebreak

$J_2$
\pagebreak

$ W(F)=c_0\iota_1(F^T F) + c_1\iota_2(F^T F) $
\pagebreak

$\iota_2$
\pagebreak

$ W(F)=c_0\iota_1(F^T F) + c_1\iota_2(F^T F) + d_0\Gamma_\mathrm{In}(\det(F))+d_1\Gamma_\mathrm{Co}(\det(F)) $
\pagebreak

$c_0,c_1,d_0,d_1$
\pagebreak

$F\rightarrow I$
\pagebreak

$\lambda,\mu$
\pagebreak

$I$
\pagebreak

$E$
\pagebreak

$\nu$
\pagebreak

$ W(F)=c\iota_1(F^T F) $
\pagebreak

$ W(F)=c\bar\iota_1(F^T F) $
\pagebreak

$\bar\iota_1$
\pagebreak

$ W(F)=c\iota_1(F^T F)+d_0\Gamma_\mathrm{In}(\det(F))+d_1\Gamma_\mathrm{Co}(\det(F)) $
\pagebreak

$ W(F)=c\bar\iota_1(F^T F)+d_0\Gamma_\mathrm{In}(\det(F))+d_1\Gamma_\mathrm{Co}(\det(F)) $
\pagebreak

$ W(F)= c_\mathrm{Cells}(\iota_1-3) + \frac{k_1}{k_2}\exp(k_2(\kappa\iota_1+(1-3\kappa)*\iota_4)^2-1) $
\pagebreak

$ \iota_1,\iota_4 $
\pagebreak

$F^T F$
\pagebreak

$(0\le\kappa\le\frac{1}{3})$
\pagebreak

$M=v\otimesv$
\pagebreak

$v$
\pagebreak

$c_\mathrm{Cells}=0.15 (\,\mathrm{kPa})$
\pagebreak

$k_1=0.8 (\,\mathrm{kPa})$
\pagebreak

$k_2=47.3$
\pagebreak

$\kappa=0.09$
\pagebreak

$ W(F)= c_\mathrm{Cells}(\iota_1-3) + \frac{k_1}{k_2}\exp(k_2(\kappa\iota_1+(1-3\kappa)*\iota_4)^2-1) + d_0\Gamma_\mathrm{Inflation}(\det(F)) + d_1\Gamma_\mathrm{Compression} $
\pagebreak

$ W(F)=c(\exp(b(\bar\iota_1-3))-1) + A(\exp(a(\bar\iota_6-1)^2)-1) $
\pagebreak

$\bar\iota_1,\bar\iota_6=\bar\iota_4$
\pagebreak

$F=I$
\pagebreak

$a=0.387 (\,\mathrm{kPa})$
\pagebreak

$ b = 23.46 $
\pagebreak

$ A = 0.584 (\,\mathrm{kPa}) $
\pagebreak

$ a = 12.43$
\pagebreak

$ W(F)=c(\exp(b(\bar\iota_1-3))-1) + A(\exp(a(\bar\iota_6-1)^2)-1) + d_0\Gamma_\mathrm{Inflation}(\det(F)) + d_1\Gamma_\mathrm{Compression} $
\pagebreak

$ W(F)=c(\exp(b(\bar\iota_1-3))-1) + A(\exp(a(\bar\iota_6-1)^2)-1) + d_0\Gamma_\mathrm{Inflation}(\det(F)) + d_1\Gamma_\mathrm{Compression}(\det(F))$
\pagebreak

$W(F)=c_0(\iota_1-3) + c_1(\iota_1-3)(\iota_2-3)$
\pagebreak

$\iota_1,\iota_2$
\pagebreak

$c_0=9.4 (\,\mathrm{kPa})$
\pagebreak

$ c_1 = 82 (\,\mathrm{kPa}) $
\pagebreak

$W(F)=c_0(\iota_1-3) + c_1(\iota_1-3)(\iota_2-3) + d_0\Gamma_\mathrm{Inflation}(\det(F)) + d_1\Gamma_\mathrm{Compression}$
\pagebreak

$(row,col)$
\pagebreak

$ A $
\pagebreak

$ A\in \mathbb{R}^{n,n} $
\pagebreak

$ n=2,3 $
\pagebreak

$(i,j)$
\pagebreak

$ (-1)^{i+j} \det(A^\#_{ij}) $
\pagebreak

$ A^\#_ij $
\pagebreak

$i$
\pagebreak

$ j $
\pagebreak

$ B $
\pagebreak

$ A^\#_{ij} $
\pagebreak

$ A\in \mathbb{R}^{3,3} $
\pagebreak

$\det(A)$
\pagebreak

$ A\in\mathbb{R}^{n,n} $
\pagebreak

$ A - \frac{\mathrm{tr}(A)}{n}I $
\pagebreak

$ J_2(\sigma)=\sqrt{\bar\sigma\negthinspace:\negthinspace\bar\sigma} $
\pagebreak

$\bar\sigma = \sigma - \frac{\mathrm{tr}(\sigma)}{n}I$
\pagebreak

$\sigma\in\mathbb{R}^{n,n}$
\pagebreak

$n$
\pagebreak

$\mathbb{R}^{n,n}$
\pagebreak

$ \|A\|^2 = A\negthinspace : \negthinspace A = \mathrm{tr}(A^TA) = \sum_{i,j} A_{ij}^2. $
\pagebreak

$ \|A\| = \sqrt{A\negthinspace : \negthinspace A }= \sqrt{\mathrm{tr}(A^TA)} = \sqrt{\sum_{i,j} A_{ij}^2}. $
\pagebreak

$\mathbb{R}^{n,m}$
\pagebreak

$\mathbb{R}^n$
\pagebreak

$m$
\pagebreak

$ \iota_4=\iota_1(AM) $
\pagebreak

$A\in\mathbb{R}^{n,n}$
\pagebreak

$M\in\mathbb{R}^{n,n}$
\pagebreak

$ \iota_5=\iota_1(A^2M) $
\pagebreak

$ \iota_6=\iota_1(AM^2) $
\pagebreak

$ \iota_4 - 1 $
\pagebreak

$ \iota_5 - 1 $
\pagebreak

$ \iota_6 - 1 $
\pagebreak

$\bar\iota_4=\iota_4\iota_3^{-1/3}$
\pagebreak

$\bar\iota_5=\iota_5\iota_3^{-2/3}$
\pagebreak

$\bar\iota_6=\iota_6\iota_3^{-1/3}$
\pagebreak

$ \bar\iota_4 - 1 $
\pagebreak

$ \bar\iota_5 - 1 $
\pagebreak

$ \bar\iota_6 - 1 $
\pagebreak

$ \bar\iota_1(A)=\iota_1\iota_3^{-1/3} $
\pagebreak

$\iota_3$
\pagebreak

$ \bar\iota_2(A)=\iota_2\iota_3^{-1/3} $
\pagebreak

$ \bar\iota_1(A) - n $
\pagebreak

$ \bar\iota_2(A) - n $
\pagebreak

$ \bar\iota_3(A) - 1 $
\pagebreak

$ \iota_1(A)=\mathrm{tr}(A) $
\pagebreak

$ \iota_2(A)=\mathrm{tr}(\mathrm{cof}(A)) $
\pagebreak

$ \iota_3(A)=\det(A) $
\pagebreak

$ \iota_1(A) - n $
\pagebreak

$ \iota_2(A) - n $
\pagebreak

$ \iota_3(A) - 1 $
\pagebreak

$scaling (invariant - offset)$
\pagebreak

$offset = dim$
\pagebreak

$offset = 1$
\pagebreak

$ F^T F $
\pagebreak

$ F $
\pagebreak

$\nabla\varphi$
\pagebreak

$F$
\pagebreak

$ F^T $
\pagebreak

$ \frac{1}{2}\left(F^T+F\right) $
\pagebreak

$\nabla u$
\pagebreak

$ \frac{1}{2}\left(F^T+F\right + F^T F) $
\pagebreak

$ F^T * F $
\pagebreak

$ F^T dF_1 + dF_1^T F $
\pagebreak

$ dF_2^T dF_1 + dF_1^T dF_2 $
\pagebreak

$ \frac{1}{2}\left(dF^T+dF\right) $
\pagebreak

$ M = v \otimes w $
\pagebreak

$ M = v \otimes v $
\pagebreak

$ f\circ g $
\pagebreak

$fg$
\pagebreak

$ af $
\pagebreak

$ f $
\pagebreak

$ a $
\pagebreak

$2^x$
\pagebreak

$ k = \frac{dividend}{divisor} $
\pagebreak

$k=-1$
\pagebreak

$k=2$
\pagebreak

$A$
\pagebreak

$A+A^T$
\pagebreak

\end{document}
